Factored the material about linear dependence, span and dimension out of the specific setting of vectors in R^n and set it up as a general theory of "matroids". These don't have all the finiteness assumptions common in matroid theory, but could be considered as "finitary" (matroid span is assumed to have finite character). The setup roughly follows Pete Clark's "Field Theory" notes, 11.4:
      http://alpha.math.uga.edu/~pete/FieldTheory.pdf

Added one more theorem WORD_SUBWORD_DUPLICATE_DUPLICATE relating
subwords and duplication, which is also now exploited inside
WORD_SIMPLE_SUBWORD_CONV.

Slightly refined the improvements to div/rem elimination made
recently, to avoid exponential blowups while preserving the ability
to deduce nonnegativity of the quotient in "easy" cases.

List of new definitions (all connected with matroids)

        matroid_basis
        matroid_dim
        matroid_dimension
        matroid_finite_dim
        matroid_finite_dimensional
        matroid_independent
        matroid_set
        matroid_span
        matroid_spanning
        matroid_subspace
        matroid_tybij
        submatroid

and theorems (all about matroids except the last one)

        FINITE_IMP_MATROID_FINITE_DIM
        FINITE_IMP_MATROID_FINITE_DIM_SPAN
        MATROID_BASES_CARD_EQ
        MATROID_BASES_FINITE
        MATROID_BASES_SIZE
        MATROID_BASIS_EQ_MAXIMAL_INDEPENDENT
        MATROID_BASIS_EQ_MINIMAL_SPANNING
        MATROID_BASIS_EXISTS
        MATROID_BASIS_EXISTS_DIM
        MATROID_BASIS_EXISTS_DIMENSION
        MATROID_BASIS_IMP_SUBSET
        MATROID_BASIS_SUBMATROID
        MATROID_CHOOSE_SUBSET
        MATROID_CHOOSE_SUBSPACE
        MATROID_CONTAINS_BASIS_DIM
        MATROID_DIMENSION_ALT
        MATROID_DIMENSION_EQ_CARD
        MATROID_DIMENSION_FINITE_LE
        MATROID_DIMENSION_GE
        MATROID_DIMENSION_GE_CARD
        MATROID_DIMENSION_GE_FINITE_CARD
        MATROID_DIMENSION_LE
        MATROID_DIMENSION_UNIQUE
        MATROID_DIM_ALT
        MATROID_DIM_BASIS
        MATROID_DIM_EMPTY
        MATROID_DIM_EQ_CARD
        MATROID_DIM_EQ_CARD_GEN
        MATROID_DIM_EQ_FINITE_CARD_EQ,MATROID_DIM_GE_FINITE_CARD_EQ
        MATROID_DIM_EQ_SPAN
        MATROID_DIM_FINITE_LE
        MATROID_DIM_GE
        MATROID_DIM_GE_CARD
        MATROID_DIM_GE_CARD_GEN
        MATROID_DIM_GE_FINITE_CARD
        MATROID_DIM_INSERT
        MATROID_DIM_LE
        MATROID_DIM_LE_CARD
        MATROID_DIM_LE_CARD_GEN
        MATROID_DIM_SET
        MATROID_DIM_SPAN
        MATROID_DIM_SPAN_EQ
        MATROID_DIM_SPAN_EQ_GEN
        MATROID_DIM_SPAN_PSUBSET
        MATROID_DIM_SPAN_SUBSET
        MATROID_DIM_SUBSET
        MATROID_DIM_SUBSET_ALT
        MATROID_DIM_UNIQUE
        MATROID_DIM_UNIQUE_ALT
        MATROID_EQ_SPANS_CARD_EQ
        MATROID_EQ_SPANS_FINITE
        MATROID_EQ_SPANS_SIZE
        MATROID_FINITE_DIM
        MATROID_FINITE_DIMENSIONAL
        MATROID_FINITE_DIMENSIONAL_ANY
        MATROID_FINITE_DIMENSIONAL_BASIS
        MATROID_FINITE_DIMENSIONAL_CONTAINS_BASIS
        MATROID_FINITE_DIMENSIONAL_DIM
        MATROID_FINITE_DIM_BASIS
        MATROID_FINITE_DIM_EMPTY
        MATROID_FINITE_DIM_FINITE
        MATROID_FINITE_DIM_IMP_SUBSET
        MATROID_FINITE_DIM_INSERT
        MATROID_FINITE_DIM_MONO
        MATROID_FINITE_DIM_SET
        MATROID_FINITE_DIM_SPAN
        MATROID_FINITE_DIM_SPAN_EQ
        MATROID_FINITE_DIM_SUBSET
        MATROID_FINITE_DIM_UNION
        MATROID_INDEPENDENT_CARD_LE_SPAN
        MATROID_INDEPENDENT_CARD_LE_SPANNING
        MATROID_INDEPENDENT_CARD_LE_SPAN_FINITE
        MATROID_INDEPENDENT_CHAIN
        MATROID_INDEPENDENT_EMPTY
        MATROID_INDEPENDENT_EXTENDS_TO_BASIS
        MATROID_INDEPENDENT_FINITARY
        MATROID_INDEPENDENT_IMP_FINITE
        MATROID_INDEPENDENT_IMP_SUBSET
        MATROID_INDEPENDENT_INSERT
        MATROID_INDEPENDENT_MONO
        MATROID_INDEPENDENT_SPANNING_FINITE
        MATROID_INDEPENDENT_SUBMATROID
        MATROID_INTERMEDIATE_BASIS
        MATROID_INTERMEDIATE_SPAN
        MATROID_LOWDIM_EXPAND_BASIS
        MATROID_LOWDIM_EXPAND_DIMENSION
        MATROID_MAXIMAL_INDEPENDENT_SUBSET_SPAN
        MATROID_SPANNING_ALT
        MATROID_SPANNING_CONTAINS_BASIS
        MATROID_SPANNING_IMP_SUBSET
        MATROID_SPANNING_PSUBSET_INDEPENDENT
        MATROID_SPANNING_SET
        MATROID_SPANNING_SUBMATROID
        MATROID_SPANNING_SUBMATROID_SELF
        MATROID_SPANNING_SUBSET_INDEPENDENT
        MATROID_SPAN_CHAIN
        MATROID_SPAN_DELETE_EQ
        MATROID_SPAN_DIM_EQ
        MATROID_SPAN_EQ
        MATROID_SPAN_EQ_SELF
        MATROID_SPAN_EQ_SET
        MATROID_SPAN_EXCHANGE_DELETE
        MATROID_SPAN_FINITARY_GEN
        MATROID_SPAN_FINITARY_MINIMAL
        MATROID_SPAN_INC
        MATROID_SPAN_INSERT_EQ
        MATROID_SPAN_INSERT_REFL
        MATROID_SPAN_INTER_SPANS
        MATROID_SPAN_INTER_SUBSET
        MATROID_SPAN_MINIMAL
        MATROID_SPAN_MONO
        MATROID_SPAN_OF_SUBSPACE
        MATROID_SPAN_PSUBSET_INDEPENDENT
        MATROID_SPAN_SET
        MATROID_SPAN_SUBSET
        MATROID_SPAN_SUBSET_EQ
        MATROID_SPAN_SUBSET_SUBSPACE
        MATROID_SPAN_SUBSPACE
        MATROID_SPAN_SUPERSET
        MATROID_SPAN_TRANS
        MATROID_SPAN_UNION_EQ
        MATROID_SPAN_UNION_SUBSET
        MATROID_STEINITZ_EXCHANGE
        MATROID_STEINITZ_EXCHANGE_ALT
        MATROID_STEINITZ_EXCHANGE_FINITE
        MATROID_SUBSET_CONTAINS_BASIS
        MATROID_SUBSPACE
        MATROID_SUBSPACE_CHAIN
        MATROID_SUBSPACE_IMP_SUBSET
        MATROID_SUBSPACE_INTER
        MATROID_SUBSPACE_INTERS
        MATROID_SUBSPACE_SET
        MATROID_SUBSPACE_SPAN
        SUBMATROID
        SUBMATROID_GEN
        SUBMATROID_SET
        SUBMATROID_SPAN
        SUBMATROID_SUBSET
        SUBSET_MATROID_SPAN
        WORD_SUBWORD_DUPLICATE_DUPLICATE

Multivariate/make_complex.ml
@@ -9,6 +9,7 @@ loadt "Library/floor.ml";;              (* Useful here and there            *)
 loadt "Multivariate/misc.ml";;          (* Background stuff                 *)
 loadt "Library/iter.ml";;               (* n-fold iteration of function     *)
 loadt "Library/grouptheory.ml";;        (* Groups, to support homology      *)
+loadt "Library/matroids.ml";;           (* Generalized linear dependence    *)
 loadt "Library/binomial.ml";;           (* For Leibniz deriv formula etc.   *)
 
 (* ------------------------------------------------------------------------- *)
